Removed TNone, added map + fold_right

code/datatypes/cuMin.v
@@ -1,4 +1,4 @@
-Require Import  Datatypes EqNat.
+Require Import  Datatypes EqNat Lists.List.
 Local Open Scope nat_scope.
 
 Notation " [ ] " := nil (format "[ ]").
@@ -47,10 +47,7 @@ Inductive ty : Type :=
   | TNat  : ty
   | TList : ty -> ty
   | TPair : ty -> ty -> ty
-  | TFun  : ty -> ty -> ty
-(*  | TFun  : list ty -> ty | list ty complicates type substitution *)
-  | TNone : ty.
-
+  | TFun  : list ty -> ty.
 
 Inductive context : Type := 
  | con : (partial_map tag) -> (partial_map ty) -> context.
@@ -135,18 +132,9 @@ Fixpoint ty_subst (k: id) (t: ty) (t': ty) : ty :=
    | TVar i      =>  if (beq_id i k) then t else TVar i
    | TBool       => TBool
    | TNat        => TNat
-   | TNone       => TNone
    | TList T     => TList (ty_subst k t T)
    | TPair TL TR => TPair (ty_subst k t TL) (ty_subst k t TR)
-(* | TFun tys => TFun (ty_subst_l tys) *)
-   | TFun  TL TR => TFun  (ty_subst k t TL) (ty_subst k t TR)
-  end.
-
-(* local definition needed? *)
-Fixpoint ty_subst_l (k: id) (t: ty) (t': list ty) : (list ty) :=
-  match t' with
-    | []          => []
-    | (t' :: t's) => (ty_subst k t t') :: (ty_subst_l k t t's)
+   | TFun tys => TFun (map (ty_subst k t) tys)
   end.
 
 Fixpoint qty_zip (qs : list quantifier) (tys : list ty) : (list (quantifier * ty)) :=
@@ -157,18 +145,28 @@ Fixpoint qty_zip (qs : list quantifier) (tys : list ty) : (list (quantifier * ty
    | (q :: qs), (ty :: tys) => (q, ty) :: (qty_zip qs tys)
   end.
 
-Fixpoint multi_ty_subst (qtys : list (quantifier * ty)) (t : ty) :=
+Fixpoint multi_ty_subst (qtys : list (quantifier * ty)) (t : ty) : option ty:=
   match qtys, t with
-   | [], t => t
-   | ((for_all id tag_star, ty) :: qtys), (TFun _ _) => TNone (* star tag doesn't allow function types *)
+   | [], t => Some t
+   | ((for_all id tag_star, ty) :: qtys), (TFun _) => None (* star tag doesn't allow function types *)
    | ((for_all id tg, ty) :: qtys), t => multi_ty_subst qtys (ty_subst id ty t)
   end.
-
-Definition func_special (fd : func_decl) (tys : list ty) : ty := 
+  
+Definition qty_subst (qty : (quantifier * ty)) (t : option ty) : option ty:=
+  match qty, t with
+   | _, None => None
+   | (for_all id tag_star, ty), Some (TFun _) => None (* star tag doesn't allow function types *)
+   | (for_all id tg, ty), Some t => Some (ty_subst id ty t)
+  end.
+  
+ Definition multi_ty_subst_alt (qtys : list (quantifier * ty)) (t : ty) : option ty := 
+  fold_right (qty_subst) (Some t) qtys.
+  
+Definition func_special (fd : func_decl) (tys : list ty) : option ty := 
   match fd with
    | (FDecl _ qs t _ _) => if (beq_nat (length qs) (length tys)) 
                            then multi_ty_subst (qty_zip qs tys) t
-                           else TNone
+                           else None
   end.
 
 Reserved Notation "Gamma '|-' t '\in' T" (at level 40).
@@ -189,16 +187,17 @@ Inductive has_type : context -> tm -> ty -> Prop :=
   | T_Nil :    forall Gamma T, 
                  Gamma |- tnil \in (TList T)
   | T_App :    forall Gamma e1 e2 T1 T2,
-                 Gamma |- e1 \in (TFun T1 T2) ->
+                 Gamma |- e1 \in (TFun [T1; T2]) ->
                  Gamma |- e2 \in T1 ->
                  Gamma |- (tapp e1 e2) \in T2
   | T_Let :    forall Gamma e1 e2 x T1 T2,
                  Gamma |- e1 \in T1 ->
                  (type_update Gamma x T1) |- e2 \in T2 ->
                  Gamma |- (tlet (tvar x) e1 e2) \in T2
-  | T_Fun :    forall Gamma P f tys,
+  | T_Fun :    forall Gamma P f tys t,
                  prog_contains P f = true ->
-                 Gamma |- (tfun tys) \in (func_special f tys) (* (tfun tys probably nonsense *)
+                 func_special f tys = Some t ->
+                 Gamma |- (tfun tys) \in t (* (tfun tys probably nonsense *)
   | T_Add :    forall Gamma e1 e2,
                  Gamma |- e1 \in TNat ->
                  Gamma |- e2 \in TNat ->
@@ -277,13 +276,13 @@ Section Examples.
   Example t6 : aContext |- tvar (Id 2) \in TVar (Id 1).
   Proof. apply T_Var. reflexivity. Qed.
   
-  Example multi_t1 : multi_ty_subst [((for_all (Id 1) tag_empty), TNat);((for_all (Id 2) tag_empty), (TList TBool))] (TFun (TFun (TVar (Id 1)) (TVar (Id 2))) TNat) = (TFun (TFun TNat (TList TBool)) TNat).
+  Example multi_t1 : multi_ty_subst [((for_all (Id 1) tag_empty), TNat);((for_all (Id 2) tag_empty), (TList TBool))] (TFun [TVar (Id 1); (TVar (Id 2)); TNat]) = Some (TFun [TNat; TList TBool; TNat]).
   Proof. reflexivity. Qed.
   
-  Example multi_t2 : multi_ty_subst [((for_all (Id 1) tag_star), (TFun TNat TBool));((for_all (Id 2) tag_empty), (TList TBool))] (TFun (TFun (TVar (Id 1)) (TVar (Id 2))) TNat) = TNone.
+  Example multi_t2 : multi_ty_subst [((for_all (Id 1) tag_star), (TFun [TNat; TBool])); ((for_all (Id 2) tag_empty), (TList TBool))] (TFun [TVar (Id 1); TVar (Id 2); TNat]) = None.
   Proof. reflexivity. Qed.
   
-  Example ty_subst1 : ty_subst (Id 1) TBool (TFun (TVar (Id 1)) (TVar (Id 1))) = TFun TBool TBool.
+  Example ty_subst1 : ty_subst (Id 1) TBool (TFun [(TVar (Id 1)); (TVar (Id 1))]) = TFun [TBool; TBool].
   Proof. reflexivity. Qed.
 
 End Examples.
